a whole lotta progress

Metrics/dafny/Metrics/runtimes/java/src/main/smithy-generated/software/amazon/cryptography/metrics/ILogger.java
@@ -1,0 +1,15 @@
+// Copyright Amazon.com Inc. or its affiliates. All Rights Reserved.
+// SPDX-License-Identifier: Apache-2.0
+// Do not modify this file. This file is machine generated, and any changes to it will be overwritten.
+package software.amazon.cryptography.metrics;
+
+import software.amazon.cryptography.metrics.model.PublishInput;
+import software.amazon.cryptography.metrics.model.PublishOutput;
+import software.amazon.cryptography.metrics.model.PutInput;
+import software.amazon.cryptography.metrics.model.PutOutput;
+
+public interface ILogger {
+  PublishOutput Publish(PublishInput input);
+
+  PutOutput Put(PutInput input);
+}
