Metrics/dafny/Metrics/runtimes/java/src/main/smithy-generated/software/amazon/cryptography/metrics/IMetricsAgent.java
@@ -1,0 +1,20 @@
+// Copyright Amazon.com Inc. or its affiliates. All Rights Reserved.
+// SPDX-License-Identifier: Apache-2.0
+// Do not modify this file. This file is machine generated, and any changes to it will be overwritten.
+package software.amazon.cryptography.metrics;
+
+import software.amazon.cryptography.metrics.model.PutCountInput;
+import software.amazon.cryptography.metrics.model.PutDateInput;
+import software.amazon.cryptography.metrics.model.PutOutput;
+import software.amazon.cryptography.metrics.model.PutPropertyInput;
+import software.amazon.cryptography.metrics.model.PutTimeInput;
+
+public interface IMetricsAgent {
+  PutOutput PutCount(PutCountInput input);
+
+  PutOutput PutDate(PutDateInput input);
+
+  PutOutput PutProperty(PutPropertyInput input);
+
+  PutOutput PutTime(PutTimeInput input);
+}
