Metrics/dafny/Metrics/runtimes/java/src/main/smithy-generated/software/amazon/cryptography/metrics/Logger.java
@@ -1,0 +1,160 @@
+// Copyright Amazon.com Inc. or its affiliates. All Rights Reserved.
+// SPDX-License-Identifier: Apache-2.0
+// Do not modify this file. This file is machine generated, and any changes to it will be overwritten.
+package software.amazon.cryptography.metrics;
+
+import Wrappers_Compile.Result;
+import java.lang.IllegalArgumentException;
+import java.lang.RuntimeException;
+import java.util.Objects;
+import software.amazon.cryptography.metrics.internaldafny.types.Error;
+import software.amazon.cryptography.metrics.model.PublishInput;
+import software.amazon.cryptography.metrics.model.PublishOutput;
+import software.amazon.cryptography.metrics.model.PutInput;
+import software.amazon.cryptography.metrics.model.PutOutput;
+
+public final class Logger implements ILogger {
+
+  private final software.amazon.cryptography.metrics.internaldafny.types.ILogger _impl;
+
+  private Logger(
+    software.amazon.cryptography.metrics.internaldafny.types.ILogger iLogger
+  ) {
+    Objects.requireNonNull(
+      iLogger,
+      "Missing value for required argument `iLogger`"
+    );
+    this._impl = iLogger;
+  }
+
+  public static Logger wrap(
+    software.amazon.cryptography.metrics.internaldafny.types.ILogger iLogger
+  ) {
+    return new Logger(iLogger);
+  }
+
+  public static <I extends ILogger> Logger wrap(I iLogger) {
+    Objects.requireNonNull(
+      iLogger,
+      "Missing value for required argument `iLogger`"
+    );
+    if (iLogger instanceof software.amazon.cryptography.metrics.Logger) {
+      return ((Logger) iLogger);
+    }
+    return Logger.wrap(new NativeWrapper(iLogger));
+  }
+
+  public software.amazon.cryptography.metrics.internaldafny.types.ILogger impl() {
+    return this._impl;
+  }
+
+  public PublishOutput Publish(PublishInput input) {
+    software.amazon.cryptography.metrics.internaldafny.types.PublishInput dafnyValue =
+      ToDafny.PublishInput(input);
+    Result<
+      software.amazon.cryptography.metrics.internaldafny.types.PublishOutput,
+      Error
+    > result = this._impl.Publish(dafnyValue);
+    if (result.is_Failure()) {
+      throw ToNative.Error(result.dtor_error());
+    }
+    return ToNative.PublishOutput(result.dtor_value());
+  }
+
+  public PutOutput Put(PutInput input) {
+    software.amazon.cryptography.metrics.internaldafny.types.PutInput dafnyValue =
+      ToDafny.PutInput(input);
+    Result<
+      software.amazon.cryptography.metrics.internaldafny.types.PutOutput,
+      Error
+    > result = this._impl.Put(dafnyValue);
+    if (result.is_Failure()) {
+      throw ToNative.Error(result.dtor_error());
+    }
+    return ToNative.PutOutput(result.dtor_value());
+  }
+
+  protected static final class NativeWrapper
+    implements
+      software.amazon.cryptography.metrics.internaldafny.types.ILogger {
+
+    protected final ILogger _impl;
+
+    NativeWrapper(ILogger nativeImpl) {
+      if (nativeImpl instanceof Logger) {
+        throw new IllegalArgumentException(
+          "Recursive wrapping is strictly forbidden."
+        );
+      }
+      this._impl = nativeImpl;
+    }
+
+    public Result<
+      software.amazon.cryptography.metrics.internaldafny.types.PublishOutput,
+      Error
+    > Publish(
+      software.amazon.cryptography.metrics.internaldafny.types.PublishInput dafnyInput
+    ) {
+      try {
+        PublishInput nativeInput = ToNative.PublishInput(dafnyInput);
+        PublishOutput nativeOutput = this._impl.Publish(nativeInput);
+        software.amazon.cryptography.metrics.internaldafny.types.PublishOutput dafnyOutput =
+          ToDafny.PublishOutput(nativeOutput);
+        return Result.create_Success(
+          software.amazon.cryptography.metrics.internaldafny.types.PublishOutput._typeDescriptor(),
+          Error._typeDescriptor(),
+          dafnyOutput
+        );
+      } catch (RuntimeException ex) {
+        return Result.create_Failure(
+          software.amazon.cryptography.metrics.internaldafny.types.PublishOutput._typeDescriptor(),
+          Error._typeDescriptor(),
+          ToDafny.Error(ex)
+        );
+      }
+    }
+
+    public Result<
+      software.amazon.cryptography.metrics.internaldafny.types.PublishOutput,
+      Error
+    > Publish_k(
+      software.amazon.cryptography.metrics.internaldafny.types.PublishInput dafnyInput
+    ) {
+      throw new RuntimeException("Not supported at this time.");
+    }
+
+    public Result<
+      software.amazon.cryptography.metrics.internaldafny.types.PutOutput,
+      Error
+    > Put(
+      software.amazon.cryptography.metrics.internaldafny.types.PutInput dafnyInput
+    ) {
+      try {
+        PutInput nativeInput = ToNative.PutInput(dafnyInput);
+        PutOutput nativeOutput = this._impl.Put(nativeInput);
+        software.amazon.cryptography.metrics.internaldafny.types.PutOutput dafnyOutput =
+          ToDafny.PutOutput(nativeOutput);
+        return Result.create_Success(
+          software.amazon.cryptography.metrics.internaldafny.types.PutOutput._typeDescriptor(),
+          Error._typeDescriptor(),
+          dafnyOutput
+        );
+      } catch (RuntimeException ex) {
+        return Result.create_Failure(
+          software.amazon.cryptography.metrics.internaldafny.types.PutOutput._typeDescriptor(),
+          Error._typeDescriptor(),
+          ToDafny.Error(ex)
+        );
+      }
+    }
+
+    public Result<
+      software.amazon.cryptography.metrics.internaldafny.types.PutOutput,
+      Error
+    > Put_k(
+      software.amazon.cryptography.metrics.internaldafny.types.PutInput dafnyInput
+    ) {
+      throw new RuntimeException("Not supported at this time.");
+    }
+  }
+}
