Metrics/dafny/Metrics/runtimes/java/src/main/smithy-generated/software/amazon/cryptography/metrics/MetricsAgent.java
@@ -1,0 +1,257 @@
+// Copyright Amazon.com Inc. or its affiliates. All Rights Reserved.
+// SPDX-License-Identifier: Apache-2.0
+// Do not modify this file. This file is machine generated, and any changes to it will be overwritten.
+package software.amazon.cryptography.metrics;
+
+import Wrappers_Compile.Result;
+import java.lang.IllegalArgumentException;
+import java.lang.RuntimeException;
+import java.util.Objects;
+import software.amazon.cryptography.metrics.internaldafny.types.Error;
+import software.amazon.cryptography.metrics.model.PutCountInput;
+import software.amazon.cryptography.metrics.model.PutDateInput;
+import software.amazon.cryptography.metrics.model.PutOutput;
+import software.amazon.cryptography.metrics.model.PutPropertyInput;
+import software.amazon.cryptography.metrics.model.PutTimeInput;
+
+public final class MetricsAgent implements IMetricsAgent {
+
+  private final software.amazon.cryptography.metrics.internaldafny.types.IMetricsAgent _impl;
+
+  private MetricsAgent(
+    software.amazon.cryptography.metrics.internaldafny.types.IMetricsAgent iMetricsAgent
+  ) {
+    Objects.requireNonNull(
+      iMetricsAgent,
+      "Missing value for required argument `iMetricsAgent`"
+    );
+    this._impl = iMetricsAgent;
+  }
+
+  public static MetricsAgent wrap(
+    software.amazon.cryptography.metrics.internaldafny.types.IMetricsAgent iMetricsAgent
+  ) {
+    return new MetricsAgent(iMetricsAgent);
+  }
+
+  public static <I extends IMetricsAgent> MetricsAgent wrap(I iMetricsAgent) {
+    Objects.requireNonNull(
+      iMetricsAgent,
+      "Missing value for required argument `iMetricsAgent`"
+    );
+    if (
+      iMetricsAgent instanceof software.amazon.cryptography.metrics.MetricsAgent
+    ) {
+      return ((MetricsAgent) iMetricsAgent);
+    }
+    return MetricsAgent.wrap(new NativeWrapper(iMetricsAgent));
+  }
+
+  public software.amazon.cryptography.metrics.internaldafny.types.IMetricsAgent impl() {
+    return this._impl;
+  }
+
+  public PutOutput PutCount(PutCountInput input) {
+    software.amazon.cryptography.metrics.internaldafny.types.PutCountInput dafnyValue =
+      ToDafny.PutCountInput(input);
+    Result<
+      software.amazon.cryptography.metrics.internaldafny.types.PutOutput,
+      Error
+    > result = this._impl.PutCount(dafnyValue);
+    if (result.is_Failure()) {
+      throw ToNative.Error(result.dtor_error());
+    }
+    return ToNative.PutOutput(result.dtor_value());
+  }
+
+  public PutOutput PutDate(PutDateInput input) {
+    software.amazon.cryptography.metrics.internaldafny.types.PutDateInput dafnyValue =
+      ToDafny.PutDateInput(input);
+    Result<
+      software.amazon.cryptography.metrics.internaldafny.types.PutOutput,
+      Error
+    > result = this._impl.PutDate(dafnyValue);
+    if (result.is_Failure()) {
+      throw ToNative.Error(result.dtor_error());
+    }
+    return ToNative.PutOutput(result.dtor_value());
+  }
+
+  public PutOutput PutProperty(PutPropertyInput input) {
+    software.amazon.cryptography.metrics.internaldafny.types.PutPropertyInput dafnyValue =
+      ToDafny.PutPropertyInput(input);
+    Result<
+      software.amazon.cryptography.metrics.internaldafny.types.PutOutput,
+      Error
+    > result = this._impl.PutProperty(dafnyValue);
+    if (result.is_Failure()) {
+      throw ToNative.Error(result.dtor_error());
+    }
+    return ToNative.PutOutput(result.dtor_value());
+  }
+
+  public PutOutput PutTime(PutTimeInput input) {
+    software.amazon.cryptography.metrics.internaldafny.types.PutTimeInput dafnyValue =
+      ToDafny.PutTimeInput(input);
+    Result<
+      software.amazon.cryptography.metrics.internaldafny.types.PutOutput,
+      Error
+    > result = this._impl.PutTime(dafnyValue);
+    if (result.is_Failure()) {
+      throw ToNative.Error(result.dtor_error());
+    }
+    return ToNative.PutOutput(result.dtor_value());
+  }
+
+  protected static final class NativeWrapper
+    implements
+      software.amazon.cryptography.metrics.internaldafny.types.IMetricsAgent {
+
+    protected final IMetricsAgent _impl;
+
+    NativeWrapper(IMetricsAgent nativeImpl) {
+      if (nativeImpl instanceof MetricsAgent) {
+        throw new IllegalArgumentException(
+          "Recursive wrapping is strictly forbidden."
+        );
+      }
+      this._impl = nativeImpl;
+    }
+
+    public Result<
+      software.amazon.cryptography.metrics.internaldafny.types.PutOutput,
+      Error
+    > PutCount(
+      software.amazon.cryptography.metrics.internaldafny.types.PutCountInput dafnyInput
+    ) {
+      try {
+        PutCountInput nativeInput = ToNative.PutCountInput(dafnyInput);
+        PutOutput nativeOutput = this._impl.PutCount(nativeInput);
+        software.amazon.cryptography.metrics.internaldafny.types.PutOutput dafnyOutput =
+          ToDafny.PutOutput(nativeOutput);
+        return Result.create_Success(
+          software.amazon.cryptography.metrics.internaldafny.types.PutOutput._typeDescriptor(),
+          Error._typeDescriptor(),
+          dafnyOutput
+        );
+      } catch (RuntimeException ex) {
+        return Result.create_Failure(
+          software.amazon.cryptography.metrics.internaldafny.types.PutOutput._typeDescriptor(),
+          Error._typeDescriptor(),
+          ToDafny.Error(ex)
+        );
+      }
+    }
+
+    public Result<
+      software.amazon.cryptography.metrics.internaldafny.types.PutOutput,
+      Error
+    > PutCount_k(
+      software.amazon.cryptography.metrics.internaldafny.types.PutCountInput dafnyInput
+    ) {
+      throw new RuntimeException("Not supported at this time.");
+    }
+
+    public Result<
+      software.amazon.cryptography.metrics.internaldafny.types.PutOutput,
+      Error
+    > PutDate(
+      software.amazon.cryptography.metrics.internaldafny.types.PutDateInput dafnyInput
+    ) {
+      try {
+        PutDateInput nativeInput = ToNative.PutDateInput(dafnyInput);
+        PutOutput nativeOutput = this._impl.PutDate(nativeInput);
+        software.amazon.cryptography.metrics.internaldafny.types.PutOutput dafnyOutput =
+          ToDafny.PutOutput(nativeOutput);
+        return Result.create_Success(
+          software.amazon.cryptography.metrics.internaldafny.types.PutOutput._typeDescriptor(),
+          Error._typeDescriptor(),
+          dafnyOutput
+        );
+      } catch (RuntimeException ex) {
+        return Result.create_Failure(
+          software.amazon.cryptography.metrics.internaldafny.types.PutOutput._typeDescriptor(),
+          Error._typeDescriptor(),
+          ToDafny.Error(ex)
+        );
+      }
+    }
+
+    public Result<
+      software.amazon.cryptography.metrics.internaldafny.types.PutOutput,
+      Error
+    > PutDate_k(
+      software.amazon.cryptography.metrics.internaldafny.types.PutDateInput dafnyInput
+    ) {
+      throw new RuntimeException("Not supported at this time.");
+    }
+
+    public Result<
+      software.amazon.cryptography.metrics.internaldafny.types.PutOutput,
+      Error
+    > PutProperty(
+      software.amazon.cryptography.metrics.internaldafny.types.PutPropertyInput dafnyInput
+    ) {
+      try {
+        PutPropertyInput nativeInput = ToNative.PutPropertyInput(dafnyInput);
+        PutOutput nativeOutput = this._impl.PutProperty(nativeInput);
+        software.amazon.cryptography.metrics.internaldafny.types.PutOutput dafnyOutput =
+          ToDafny.PutOutput(nativeOutput);
+        return Result.create_Success(
+          software.amazon.cryptography.metrics.internaldafny.types.PutOutput._typeDescriptor(),
+          Error._typeDescriptor(),
+          dafnyOutput
+        );
+      } catch (RuntimeException ex) {
+        return Result.create_Failure(
+          software.amazon.cryptography.metrics.internaldafny.types.PutOutput._typeDescriptor(),
+          Error._typeDescriptor(),
+          ToDafny.Error(ex)
+        );
+      }
+    }
+
+    public Result<
+      software.amazon.cryptography.metrics.internaldafny.types.PutOutput,
+      Error
+    > PutProperty_k(
+      software.amazon.cryptography.metrics.internaldafny.types.PutPropertyInput dafnyInput
+    ) {
+      throw new RuntimeException("Not supported at this time.");
+    }
+
+    public Result<
+      software.amazon.cryptography.metrics.internaldafny.types.PutOutput,
+      Error
+    > PutTime(
+      software.amazon.cryptography.metrics.internaldafny.types.PutTimeInput dafnyInput
+    ) {
+      try {
+        PutTimeInput nativeInput = ToNative.PutTimeInput(dafnyInput);
+        PutOutput nativeOutput = this._impl.PutTime(nativeInput);
+        software.amazon.cryptography.metrics.internaldafny.types.PutOutput dafnyOutput =
+          ToDafny.PutOutput(nativeOutput);
+        return Result.create_Success(
+          software.amazon.cryptography.metrics.internaldafny.types.PutOutput._typeDescriptor(),
+          Error._typeDescriptor(),
+          dafnyOutput
+        );
+      } catch (RuntimeException ex) {
+        return Result.create_Failure(
+          software.amazon.cryptography.metrics.internaldafny.types.PutOutput._typeDescriptor(),
+          Error._typeDescriptor(),
+          ToDafny.Error(ex)
+        );
+      }
+    }
+
+    public Result<
+      software.amazon.cryptography.metrics.internaldafny.types.PutOutput,
+      Error
+    > PutTime_k(
+      software.amazon.cryptography.metrics.internaldafny.types.PutTimeInput dafnyInput
+    ) {
+      throw new RuntimeException("Not supported at this time.");
+    }
+  }
+}
