Metrics/dafny/Metrics/runtimes/java/src/main/smithy-generated/software/amazon/cryptography/metrics/ToNative.java
@@ -1,0 +1,351 @@
+// Copyright Amazon.com Inc. or its affiliates. All Rights Reserved.
+// SPDX-License-Identifier: Apache-2.0
+// Do not modify this file. This file is machine generated, and any changes to it will be overwritten.
+package software.amazon.cryptography.metrics;
+
+import dafny.DafnySequence;
+import java.lang.RuntimeException;
+import java.util.List;
+import software.amazon.cryptography.metrics.internaldafny.types.Error;
+import software.amazon.cryptography.metrics.internaldafny.types.Error_CollectionOfErrors;
+import software.amazon.cryptography.metrics.internaldafny.types.Error_MetricsPublishError;
+import software.amazon.cryptography.metrics.internaldafny.types.Error_MetricsPutError;
+import software.amazon.cryptography.metrics.internaldafny.types.Error_MetricsServiceError;
+import software.amazon.cryptography.metrics.internaldafny.types.Error_Opaque;
+import software.amazon.cryptography.metrics.internaldafny.types.Error_OpaqueWithText;
+import software.amazon.cryptography.metrics.internaldafny.types.IAwsCryptographicMetricsClient;
+import software.amazon.cryptography.metrics.model.CollectionOfErrors;
+import software.amazon.cryptography.metrics.model.CreateLoggerOutput;
+import software.amazon.cryptography.metrics.model.CreateMetricsAgentInput;
+import software.amazon.cryptography.metrics.model.CreateMetricsAgentOutput;
+import software.amazon.cryptography.metrics.model.CreateTextLoggerInput;
+import software.amazon.cryptography.metrics.model.CreateTextMetricsAgentInput;
+import software.amazon.cryptography.metrics.model.MetricsConfig;
+import software.amazon.cryptography.metrics.model.MetricsPublishError;
+import software.amazon.cryptography.metrics.model.MetricsPutError;
+import software.amazon.cryptography.metrics.model.MetricsServiceError;
+import software.amazon.cryptography.metrics.model.OpaqueError;
+import software.amazon.cryptography.metrics.model.OpaqueWithTextError;
+import software.amazon.cryptography.metrics.model.PublishInput;
+import software.amazon.cryptography.metrics.model.PublishOutput;
+import software.amazon.cryptography.metrics.model.PutCountInput;
+import software.amazon.cryptography.metrics.model.PutDateInput;
+import software.amazon.cryptography.metrics.model.PutInput;
+import software.amazon.cryptography.metrics.model.PutOutput;
+import software.amazon.cryptography.metrics.model.PutPropertyInput;
+import software.amazon.cryptography.metrics.model.PutTimeInput;
+
+public class ToNative {
+
+  public static OpaqueError Error(Error_Opaque dafnyValue) {
+    OpaqueError.Builder nativeBuilder = OpaqueError.builder();
+    nativeBuilder.obj(dafnyValue.dtor_obj());
+    return nativeBuilder.build();
+  }
+
+  public static OpaqueWithTextError Error(Error_OpaqueWithText dafnyValue) {
+    OpaqueWithTextError.Builder nativeBuilder = OpaqueWithTextError.builder();
+    nativeBuilder.obj(dafnyValue.dtor_obj());
+    nativeBuilder.objMessage(
+      software.amazon.smithy.dafny.conversion.ToNative.Simple.String(
+        dafnyValue.dtor_objMessage()
+      )
+    );
+    return nativeBuilder.build();
+  }
+
+  public static CollectionOfErrors Error(Error_CollectionOfErrors dafnyValue) {
+    CollectionOfErrors.Builder nativeBuilder = CollectionOfErrors.builder();
+    nativeBuilder.list(
+      software.amazon.smithy.dafny.conversion.ToNative.Aggregate.GenericToList(
+        dafnyValue.dtor_list(),
+        ToNative::Error
+      )
+    );
+    nativeBuilder.message(
+      software.amazon.smithy.dafny.conversion.ToNative.Simple.String(
+        dafnyValue.dtor_message()
+      )
+    );
+    return nativeBuilder.build();
+  }
+
+  public static MetricsPublishError Error(
+    Error_MetricsPublishError dafnyValue
+  ) {
+    MetricsPublishError.Builder nativeBuilder = MetricsPublishError.builder();
+    nativeBuilder.message(
+      software.amazon.smithy.dafny.conversion.ToNative.Simple.String(
+        dafnyValue.dtor_message()
+      )
+    );
+    return nativeBuilder.build();
+  }
+
+  public static MetricsPutError Error(Error_MetricsPutError dafnyValue) {
+    MetricsPutError.Builder nativeBuilder = MetricsPutError.builder();
+    nativeBuilder.message(
+      software.amazon.smithy.dafny.conversion.ToNative.Simple.String(
+        dafnyValue.dtor_message()
+      )
+    );
+    return nativeBuilder.build();
+  }
+
+  public static MetricsServiceError Error(
+    Error_MetricsServiceError dafnyValue
+  ) {
+    MetricsServiceError.Builder nativeBuilder = MetricsServiceError.builder();
+    nativeBuilder.message(
+      software.amazon.smithy.dafny.conversion.ToNative.Simple.String(
+        dafnyValue.dtor_message()
+      )
+    );
+    return nativeBuilder.build();
+  }
+
+  public static RuntimeException Error(Error dafnyValue) {
+    if (dafnyValue.is_MetricsPublishError()) {
+      return ToNative.Error((Error_MetricsPublishError) dafnyValue);
+    }
+    if (dafnyValue.is_MetricsPutError()) {
+      return ToNative.Error((Error_MetricsPutError) dafnyValue);
+    }
+    if (dafnyValue.is_MetricsServiceError()) {
+      return ToNative.Error((Error_MetricsServiceError) dafnyValue);
+    }
+    if (dafnyValue.is_Opaque()) {
+      return ToNative.Error((Error_Opaque) dafnyValue);
+    }
+    if (dafnyValue.is_OpaqueWithText()) {
+      return ToNative.Error((Error_OpaqueWithText) dafnyValue);
+    }
+    if (dafnyValue.is_CollectionOfErrors()) {
+      return ToNative.Error((Error_CollectionOfErrors) dafnyValue);
+    }
+    OpaqueError.Builder nativeBuilder = OpaqueError.builder();
+    nativeBuilder.obj(dafnyValue);
+    return nativeBuilder.build();
+  }
+
+  public static CreateLoggerOutput CreateLoggerOutput(
+    software.amazon.cryptography.metrics.internaldafny.types.CreateLoggerOutput dafnyValue
+  ) {
+    CreateLoggerOutput.Builder nativeBuilder = CreateLoggerOutput.builder();
+    nativeBuilder.logger(ToNative.Logger(dafnyValue.dtor_logger()));
+    return nativeBuilder.build();
+  }
+
+  public static CreateMetricsAgentInput CreateMetricsAgentInput(
+    software.amazon.cryptography.metrics.internaldafny.types.CreateMetricsAgentInput dafnyValue
+  ) {
+    CreateMetricsAgentInput.Builder nativeBuilder =
+      CreateMetricsAgentInput.builder();
+    nativeBuilder.metricsAgents(
+      ToNative.MetricsAgentList(dafnyValue.dtor_metricsAgents())
+    );
+    return nativeBuilder.build();
+  }
+
+  public static CreateMetricsAgentOutput CreateMetricsAgentOutput(
+    software.amazon.cryptography.metrics.internaldafny.types.CreateMetricsAgentOutput dafnyValue
+  ) {
+    CreateMetricsAgentOutput.Builder nativeBuilder =
+      CreateMetricsAgentOutput.builder();
+    nativeBuilder.metricsAgent(
+      ToNative.MetricsAgent(dafnyValue.dtor_metricsAgent())
+    );
+    return nativeBuilder.build();
+  }
+
+  public static CreateTextLoggerInput CreateTextLoggerInput(
+    software.amazon.cryptography.metrics.internaldafny.types.CreateTextLoggerInput dafnyValue
+  ) {
+    CreateTextLoggerInput.Builder nativeBuilder =
+      CreateTextLoggerInput.builder();
+    if (dafnyValue.dtor_fileName().is_Some()) {
+      nativeBuilder.fileName(
+        software.amazon.smithy.dafny.conversion.ToNative.Simple.String(
+          dafnyValue.dtor_fileName().dtor_value()
+        )
+      );
+    }
+    return nativeBuilder.build();
+  }
+
+  public static CreateTextMetricsAgentInput CreateTextMetricsAgentInput(
+    software.amazon.cryptography.metrics.internaldafny.types.CreateTextMetricsAgentInput dafnyValue
+  ) {
+    CreateTextMetricsAgentInput.Builder nativeBuilder =
+      CreateTextMetricsAgentInput.builder();
+    nativeBuilder.fileName(
+      software.amazon.smithy.dafny.conversion.ToNative.Simple.String(
+        dafnyValue.dtor_fileName()
+      )
+    );
+    return nativeBuilder.build();
+  }
+
+  public static MetricsConfig MetricsConfig(
+    software.amazon.cryptography.metrics.internaldafny.types.MetricsConfig dafnyValue
+  ) {
+    MetricsConfig.Builder nativeBuilder = MetricsConfig.builder();
+    return nativeBuilder.build();
+  }
+
+  public static PublishInput PublishInput(
+    software.amazon.cryptography.metrics.internaldafny.types.PublishInput dafnyValue
+  ) {
+    PublishInput.Builder nativeBuilder = PublishInput.builder();
+    return nativeBuilder.build();
+  }
+
+  public static PublishOutput PublishOutput(
+    software.amazon.cryptography.metrics.internaldafny.types.PublishOutput dafnyValue
+  ) {
+    PublishOutput.Builder nativeBuilder = PublishOutput.builder();
+    return nativeBuilder.build();
+  }
+
+  public static PutCountInput PutCountInput(
+    software.amazon.cryptography.metrics.internaldafny.types.PutCountInput dafnyValue
+  ) {
+    PutCountInput.Builder nativeBuilder = PutCountInput.builder();
+    nativeBuilder.description(
+      software.amazon.smithy.dafny.conversion.ToNative.Simple.String(
+        dafnyValue.dtor_description()
+      )
+    );
+    nativeBuilder.count((dafnyValue.dtor_count()));
+    if (dafnyValue.dtor_transactionId().is_Some()) {
+      nativeBuilder.transactionId(
+        software.amazon.smithy.dafny.conversion.ToNative.Simple.String(
+          dafnyValue.dtor_transactionId().dtor_value()
+        )
+      );
+    }
+    return nativeBuilder.build();
+  }
+
+  public static PutDateInput PutDateInput(
+    software.amazon.cryptography.metrics.internaldafny.types.PutDateInput dafnyValue
+  ) {
+    PutDateInput.Builder nativeBuilder = PutDateInput.builder();
+    nativeBuilder.description(
+      software.amazon.smithy.dafny.conversion.ToNative.Simple.String(
+        dafnyValue.dtor_description()
+      )
+    );
+    nativeBuilder.date(
+      software.amazon.smithy.dafny.conversion.ToNative.Simple.Date(
+        dafnyValue.dtor_date()
+      )
+    );
+    if (dafnyValue.dtor_transactionId().is_Some()) {
+      nativeBuilder.transactionId(
+        software.amazon.smithy.dafny.conversion.ToNative.Simple.String(
+          dafnyValue.dtor_transactionId().dtor_value()
+        )
+      );
+    }
+    return nativeBuilder.build();
+  }
+
+  public static PutInput PutInput(
+    software.amazon.cryptography.metrics.internaldafny.types.PutInput dafnyValue
+  ) {
+    PutInput.Builder nativeBuilder = PutInput.builder();
+    nativeBuilder.message(
+      software.amazon.smithy.dafny.conversion.ToNative.Simple.String(
+        dafnyValue.dtor_message()
+      )
+    );
+    return nativeBuilder.build();
+  }
+
+  public static PutOutput PutOutput(
+    software.amazon.cryptography.metrics.internaldafny.types.PutOutput dafnyValue
+  ) {
+    PutOutput.Builder nativeBuilder = PutOutput.builder();
+    return nativeBuilder.build();
+  }
+
+  public static PutPropertyInput PutPropertyInput(
+    software.amazon.cryptography.metrics.internaldafny.types.PutPropertyInput dafnyValue
+  ) {
+    PutPropertyInput.Builder nativeBuilder = PutPropertyInput.builder();
+    nativeBuilder.description(
+      software.amazon.smithy.dafny.conversion.ToNative.Simple.String(
+        dafnyValue.dtor_description()
+      )
+    );
+    nativeBuilder.value(
+      software.amazon.smithy.dafny.conversion.ToNative.Simple.String(
+        dafnyValue.dtor_value()
+      )
+    );
+    if (dafnyValue.dtor_transactionId().is_Some()) {
+      nativeBuilder.transactionId(
+        software.amazon.smithy.dafny.conversion.ToNative.Simple.String(
+          dafnyValue.dtor_transactionId().dtor_value()
+        )
+      );
+    }
+    return nativeBuilder.build();
+  }
+
+  public static PutTimeInput PutTimeInput(
+    software.amazon.cryptography.metrics.internaldafny.types.PutTimeInput dafnyValue
+  ) {
+    PutTimeInput.Builder nativeBuilder = PutTimeInput.builder();
+    nativeBuilder.description(
+      software.amazon.smithy.dafny.conversion.ToNative.Simple.String(
+        dafnyValue.dtor_description()
+      )
+    );
+    nativeBuilder.duration((dafnyValue.dtor_duration()));
+    if (dafnyValue.dtor_transactionId().is_Some()) {
+      nativeBuilder.transactionId(
+        software.amazon.smithy.dafny.conversion.ToNative.Simple.String(
+          dafnyValue.dtor_transactionId().dtor_value()
+        )
+      );
+    }
+    return nativeBuilder.build();
+  }
+
+  public static List<IMetricsAgent> MetricsAgentList(
+    DafnySequence<
+      ? extends software.amazon.cryptography.metrics.internaldafny.types.IMetricsAgent
+    > dafnyValue
+  ) {
+    return software.amazon.smithy.dafny.conversion.ToNative.Aggregate.GenericToList(
+      dafnyValue,
+      software.amazon.cryptography.metrics.ToNative::MetricsAgent
+    );
+  }
+
+  public static ILogger Logger(
+    software.amazon.cryptography.metrics.internaldafny.types.ILogger dafnyValue
+  ) {
+    if (dafnyValue instanceof Logger.NativeWrapper) {
+      return ((Logger.NativeWrapper) dafnyValue)._impl;
+    }
+    return Logger.wrap(dafnyValue);
+  }
+
+  public static IMetricsAgent MetricsAgent(
+    software.amazon.cryptography.metrics.internaldafny.types.IMetricsAgent dafnyValue
+  ) {
+    if (dafnyValue instanceof MetricsAgent.NativeWrapper) {
+      return ((MetricsAgent.NativeWrapper) dafnyValue)._impl;
+    }
+    return MetricsAgent.wrap(dafnyValue);
+  }
+
+  public static Metrics AwsCryptographicMetrics(
+    IAwsCryptographicMetricsClient dafnyValue
+  ) {
+    return new Metrics(dafnyValue);
+  }
+}
