Metrics/dafny/Metrics/runtimes/java/src/main/smithy-generated/software/amazon/cryptography/metrics/model/CreateLoggerOutput.java
@@ -1,0 +1,66 @@
+// Copyright Amazon.com Inc. or its affiliates. All Rights Reserved.
+// SPDX-License-Identifier: Apache-2.0
+// Do not modify this file. This file is machine generated, and any changes to it will be overwritten.
+package software.amazon.cryptography.metrics.model;
+
+import java.util.Objects;
+import software.amazon.cryptography.metrics.ILogger;
+import software.amazon.cryptography.metrics.Logger;
+
+public class CreateLoggerOutput {
+
+  private final ILogger logger;
+
+  protected CreateLoggerOutput(BuilderImpl builder) {
+    this.logger = builder.logger();
+  }
+
+  public ILogger logger() {
+    return this.logger;
+  }
+
+  public Builder toBuilder() {
+    return new BuilderImpl(this);
+  }
+
+  public static Builder builder() {
+    return new BuilderImpl();
+  }
+
+  public interface Builder {
+    Builder logger(ILogger logger);
+
+    ILogger logger();
+
+    CreateLoggerOutput build();
+  }
+
+  static class BuilderImpl implements Builder {
+
+    protected ILogger logger;
+
+    protected BuilderImpl() {}
+
+    protected BuilderImpl(CreateLoggerOutput model) {
+      this.logger = model.logger();
+    }
+
+    public Builder logger(ILogger logger) {
+      this.logger = Logger.wrap(logger);
+      return this;
+    }
+
+    public ILogger logger() {
+      return this.logger;
+    }
+
+    public CreateLoggerOutput build() {
+      if (Objects.isNull(this.logger())) {
+        throw new IllegalArgumentException(
+          "Missing value for required field `logger`"
+        );
+      }
+      return new CreateLoggerOutput(this);
+    }
+  }
+}
