Metrics/dafny/Metrics/runtimes/java/src/main/smithy-generated/software/amazon/cryptography/metrics/model/CreateMetricsAgentInput.java
@@ -1,0 +1,66 @@
+// Copyright Amazon.com Inc. or its affiliates. All Rights Reserved.
+// SPDX-License-Identifier: Apache-2.0
+// Do not modify this file. This file is machine generated, and any changes to it will be overwritten.
+package software.amazon.cryptography.metrics.model;
+
+import java.util.List;
+import java.util.Objects;
+import software.amazon.cryptography.metrics.IMetricsAgent;
+
+public class CreateMetricsAgentInput {
+
+  private final List<IMetricsAgent> metricsAgents;
+
+  protected CreateMetricsAgentInput(BuilderImpl builder) {
+    this.metricsAgents = builder.metricsAgents();
+  }
+
+  public List<IMetricsAgent> metricsAgents() {
+    return this.metricsAgents;
+  }
+
+  public Builder toBuilder() {
+    return new BuilderImpl(this);
+  }
+
+  public static Builder builder() {
+    return new BuilderImpl();
+  }
+
+  public interface Builder {
+    Builder metricsAgents(List<IMetricsAgent> metricsAgents);
+
+    List<IMetricsAgent> metricsAgents();
+
+    CreateMetricsAgentInput build();
+  }
+
+  static class BuilderImpl implements Builder {
+
+    protected List<IMetricsAgent> metricsAgents;
+
+    protected BuilderImpl() {}
+
+    protected BuilderImpl(CreateMetricsAgentInput model) {
+      this.metricsAgents = model.metricsAgents();
+    }
+
+    public Builder metricsAgents(List<IMetricsAgent> metricsAgents) {
+      this.metricsAgents = metricsAgents;
+      return this;
+    }
+
+    public List<IMetricsAgent> metricsAgents() {
+      return this.metricsAgents;
+    }
+
+    public CreateMetricsAgentInput build() {
+      if (Objects.isNull(this.metricsAgents())) {
+        throw new IllegalArgumentException(
+          "Missing value for required field `metricsAgents`"
+        );
+      }
+      return new CreateMetricsAgentInput(this);
+    }
+  }
+}
