Metrics/dafny/Metrics/runtimes/java/src/main/smithy-generated/software/amazon/cryptography/metrics/model/CreateTextLoggerInput.java
@@ -1,0 +1,57 @@
+// Copyright Amazon.com Inc. or its affiliates. All Rights Reserved.
+// SPDX-License-Identifier: Apache-2.0
+// Do not modify this file. This file is machine generated, and any changes to it will be overwritten.
+package software.amazon.cryptography.metrics.model;
+
+public class CreateTextLoggerInput {
+
+  private final String fileName;
+
+  protected CreateTextLoggerInput(BuilderImpl builder) {
+    this.fileName = builder.fileName();
+  }
+
+  public String fileName() {
+    return this.fileName;
+  }
+
+  public Builder toBuilder() {
+    return new BuilderImpl(this);
+  }
+
+  public static Builder builder() {
+    return new BuilderImpl();
+  }
+
+  public interface Builder {
+    Builder fileName(String fileName);
+
+    String fileName();
+
+    CreateTextLoggerInput build();
+  }
+
+  static class BuilderImpl implements Builder {
+
+    protected String fileName;
+
+    protected BuilderImpl() {}
+
+    protected BuilderImpl(CreateTextLoggerInput model) {
+      this.fileName = model.fileName();
+    }
+
+    public Builder fileName(String fileName) {
+      this.fileName = fileName;
+      return this;
+    }
+
+    public String fileName() {
+      return this.fileName;
+    }
+
+    public CreateTextLoggerInput build() {
+      return new CreateTextLoggerInput(this);
+    }
+  }
+}
