Metrics/dafny/Metrics/runtimes/java/src/main/smithy-generated/software/amazon/cryptography/metrics/model/PublishOutput.java
@@ -1,0 +1,32 @@
+// Copyright Amazon.com Inc. or its affiliates. All Rights Reserved.
+// SPDX-License-Identifier: Apache-2.0
+// Do not modify this file. This file is machine generated, and any changes to it will be overwritten.
+package software.amazon.cryptography.metrics.model;
+
+public class PublishOutput {
+
+  protected PublishOutput(BuilderImpl builder) {}
+
+  public Builder toBuilder() {
+    return new BuilderImpl(this);
+  }
+
+  public static Builder builder() {
+    return new BuilderImpl();
+  }
+
+  public interface Builder {
+    PublishOutput build();
+  }
+
+  static class BuilderImpl implements Builder {
+
+    protected BuilderImpl() {}
+
+    protected BuilderImpl(PublishOutput model) {}
+
+    public PublishOutput build() {
+      return new PublishOutput(this);
+    }
+  }
+}
