Metrics/dafny/Metrics/runtimes/java/src/main/smithy-generated/software/amazon/cryptography/metrics/model/PutDateInput.java
@@ -1,0 +1,116 @@
+// Copyright Amazon.com Inc. or its affiliates. All Rights Reserved.
+// SPDX-License-Identifier: Apache-2.0
+// Do not modify this file. This file is machine generated, and any changes to it will be overwritten.
+package software.amazon.cryptography.metrics.model;
+
+import java.time.Instant;
+import java.util.Objects;
+
+public class PutDateInput {
+
+  private final String description;
+
+  private final Instant date;
+
+  private final String transactionId;
+
+  protected PutDateInput(BuilderImpl builder) {
+    this.description = builder.description();
+    this.date = builder.date();
+    this.transactionId = builder.transactionId();
+  }
+
+  public String description() {
+    return this.description;
+  }
+
+  public Instant date() {
+    return this.date;
+  }
+
+  public String transactionId() {
+    return this.transactionId;
+  }
+
+  public Builder toBuilder() {
+    return new BuilderImpl(this);
+  }
+
+  public static Builder builder() {
+    return new BuilderImpl();
+  }
+
+  public interface Builder {
+    Builder description(String description);
+
+    String description();
+
+    Builder date(Instant date);
+
+    Instant date();
+
+    Builder transactionId(String transactionId);
+
+    String transactionId();
+
+    PutDateInput build();
+  }
+
+  static class BuilderImpl implements Builder {
+
+    protected String description;
+
+    protected Instant date;
+
+    protected String transactionId;
+
+    protected BuilderImpl() {}
+
+    protected BuilderImpl(PutDateInput model) {
+      this.description = model.description();
+      this.date = model.date();
+      this.transactionId = model.transactionId();
+    }
+
+    public Builder description(String description) {
+      this.description = description;
+      return this;
+    }
+
+    public String description() {
+      return this.description;
+    }
+
+    public Builder date(Instant date) {
+      this.date = date;
+      return this;
+    }
+
+    public Instant date() {
+      return this.date;
+    }
+
+    public Builder transactionId(String transactionId) {
+      this.transactionId = transactionId;
+      return this;
+    }
+
+    public String transactionId() {
+      return this.transactionId;
+    }
+
+    public PutDateInput build() {
+      if (Objects.isNull(this.description())) {
+        throw new IllegalArgumentException(
+          "Missing value for required field `description`"
+        );
+      }
+      if (Objects.isNull(this.date())) {
+        throw new IllegalArgumentException(
+          "Missing value for required field `date`"
+        );
+      }
+      return new PutDateInput(this);
+    }
+  }
+}
