Metrics/dafny/Metrics/runtimes/java/src/main/smithy-generated/software/amazon/cryptography/metrics/model/PutInput.java
@@ -1,0 +1,64 @@
+// Copyright Amazon.com Inc. or its affiliates. All Rights Reserved.
+// SPDX-License-Identifier: Apache-2.0
+// Do not modify this file. This file is machine generated, and any changes to it will be overwritten.
+package software.amazon.cryptography.metrics.model;
+
+import java.util.Objects;
+
+public class PutInput {
+
+  private final String message;
+
+  protected PutInput(BuilderImpl builder) {
+    this.message = builder.message();
+  }
+
+  public String message() {
+    return this.message;
+  }
+
+  public Builder toBuilder() {
+    return new BuilderImpl(this);
+  }
+
+  public static Builder builder() {
+    return new BuilderImpl();
+  }
+
+  public interface Builder {
+    Builder message(String message);
+
+    String message();
+
+    PutInput build();
+  }
+
+  static class BuilderImpl implements Builder {
+
+    protected String message;
+
+    protected BuilderImpl() {}
+
+    protected BuilderImpl(PutInput model) {
+      this.message = model.message();
+    }
+
+    public Builder message(String message) {
+      this.message = message;
+      return this;
+    }
+
+    public String message() {
+      return this.message;
+    }
+
+    public PutInput build() {
+      if (Objects.isNull(this.message())) {
+        throw new IllegalArgumentException(
+          "Missing value for required field `message`"
+        );
+      }
+      return new PutInput(this);
+    }
+  }
+}
