Metrics/dafny/Metrics/src/MetricsAgent.dfy
@@ -1,0 +1,23 @@
+// Copyright Amazon.com Inc. or its affiliates. All Rights Reserved.
+// SPDX-License-Identifier: Apache-2.0
+
+include "../Model/AwsCryptographyMetricsTypes.dfy"
+
+module {:options "/functionSyntax:4" } MetricsAgent {
+  import opened Wrappers
+  import Types = AwsCryptographyMetricsTypes
+
+  trait {:termination false} VerifiableInterface
+    extends Types.IMetricsAgent
+  {
+
+    ghost predicate PutCountEnsuresPublicly(input: Types.PutCountInput , output: Result<Types.PutOutput, Types.Error>)
+      : (outcome: bool)
+    ghost predicate PutDateEnsuresPublicly(input: Types.PutDateInput , output: Result<Types.PutOutput, Types.Error>)
+      : (outcome: bool)
+    ghost predicate PutTimeEnsuresPublicly(input: Types.PutTimeInput , output: Result<Types.PutOutput, Types.Error>)
+      : (outcome: bool)
+    ghost predicate PutPropertyEnsuresPublicly(input: Types.PutPropertyInput , output: Result<Types.PutOutput, Types.Error>)
+      : (outcome: bool)
+  }
+}
