Metrics/dafny/Metrics/src/MetricsAgentText.dfy
@@ -1,0 +1,167 @@
+// Copyright Amazon.com Inc. or its affiliates. All Rights Reserved.
+// SPDX-License-Identifier: Apache-2.0
+
+include "../Model/AwsCryptographyMetricsTypes.dfy"
+include "MetricsAgent.dfy"
+
+
+module MetricsAgentText {
+  import opened Types = AwsCryptographyMetricsTypes
+  import opened Wrappers
+  import opened StandardLibrary.UInt
+  import MetricsAgent
+
+  class TextLogger
+    extends MetricsAgent.VerifiableInterface
+  {
+    const fileName: string
+
+    predicate ValidState()
+      ensures ValidState() ==> History in Modifies
+    {
+      && History in Modifies
+    }
+
+    constructor {:extern} {:axiom} (
+      fileName: string
+    )
+      requires |fileName| > 0
+      ensures ValidState()
+      ensures fresh (Modifies) && fresh(History) 
+    {
+      this.fileName := fileName;
+      History := new Types.IMetricsAgentCallHistory();
+      Modifies := {History};
+    }
+
+    predicate PutCountEnsuresPublicly(input: Types.PutCountInput , output: Result<Types.PutOutput, Types.Error>)
+      : (outcome: bool)
+    {
+      && output.Success?
+    }
+    
+    method PutCount' ( input: PutCountInput )
+      returns (output: Result<PutOutput, Error>)
+      requires
+        && ValidState()
+      modifies Modifies - {History}
+      // Dafny will skip type parameters when generating a default decreases clause.
+      decreases Modifies - {History}
+      ensures
+        && ValidState()
+      ensures PutCountEnsuresPublicly(input, output)
+      ensures unchanged(History)
+    {
+      var _ := ExternPutCount(
+        input.description,
+        input.count,
+        input.transactionId
+      );
+
+      return Success(PutOutput());
+    }
+
+    predicate PutDateEnsuresPublicly(input: Types.PutDateInput , output: Result<Types.PutOutput, Types.Error>)
+      : (outcome: bool)
+    {
+      && output.Success?
+    }
+    
+    method PutDate' ( input: PutDateInput )
+      returns (output: Result<PutOutput, Error>)
+      requires
+        && ValidState()
+      modifies Modifies - {History}
+      // Dafny will skip type parameters when generating a default decreases clause.
+      decreases Modifies - {History}
+      ensures
+        && ValidState()
+      ensures PutDateEnsuresPublicly(input, output)
+      ensures unchanged(History)
+    {
+      var _ := ExternPutDate(
+        input.description,
+        input.date,
+        input.transactionId
+      );
+      return Success(PutOutput());
+    }
+    
+    predicate PutTimeEnsuresPublicly(input: Types.PutTimeInput , output: Result<Types.PutOutput, Types.Error>)
+      : (outcome: bool)
+    {
+      && output.Success?
+    }
+    
+    method PutTime' ( input: PutTimeInput )
+      returns (output: Result<PutOutput, Error>)
+      requires
+        && ValidState()
+      modifies Modifies - {History}
+      // Dafny will skip type parameters when generating a default decreases clause.
+      decreases Modifies - {History}
+      ensures
+        && ValidState()
+      ensures PutTimeEnsuresPublicly(input, output)
+      ensures unchanged(History)
+    {
+      var _ := ExternPutTime(
+        input.description,
+        input.duration,
+        input.transactionId
+      );
+      return Success(PutOutput());
+    }
+
+    predicate PutPropertyEnsuresPublicly(input: Types.PutPropertyInput , output: Result<Types.PutOutput, Types.Error>)
+      : (outcome: bool)
+    {
+      && output.Success?
+    }
+    method PutProperty' ( input: PutPropertyInput )
+      returns (output: Result<PutOutput, Error>)
+      requires
+        && ValidState()
+      modifies Modifies - {History}
+      // Dafny will skip type parameters when generating a default decreases clause.
+      decreases Modifies - {History}
+      ensures
+        && ValidState()
+      ensures PutPropertyEnsuresPublicly(input, output)
+      ensures unchanged(History)
+      {
+        var _ := ExternPutProperty(
+          input.description,
+          input.value,
+          input.transactionId
+        );
+        return Success(PutOutput());
+      }
+  }
+
+  // Externs
+  method {:extern "MetricsAgent.TextLogger", "PutCount"} ExternPutCount(
+    description: string ,
+    count: int64 ,
+    transactionId: Option<string> := Option.None
+  ) returns (res: bool)
+  
+  method {:extern "MetricsAgent.TextLogger", "PutDate"} ExternPutDate(
+    description: string ,
+    date: string ,
+    transactionId: Option<string> := Option.None
+  ) returns (res: bool)
+  
+  method {:extern "MetricsAgent.TextLogger", "PutTime"} ExternPutTime(
+    description: string ,
+    duration: int64 ,
+    transactionId: Option<string> := Option.None
+  ) returns (res: bool)
+  
+  method {:extern "MetricsAgent.TextLogger", "PutProperty"} ExternPutProperty(
+    description: string ,
+    value: string ,
+    transactionId: Option<string> := Option.None
+  ) returns (res: bool)
+
+}
