Metrics/dafny/Metrics/test/TestMetricsAgentText.dfy
@@ -1,0 +1,25 @@
+// Copyright Amazon.com Inc. or its affiliates. All Rights Reserved.
+// SPDX-License-Identifier: Apache-2.0
+
+include "../src/Index.dfy"
+
+module TestMetricsAgentText {
+  import opened Wrappers
+  import Types = AwsCryptographyMetricsTypes
+  import Metrics
+  import UUID
+
+  method {:test} TestCreateTextMetricsAgent()
+  {
+    var metrics :- expect Metrics.MetricsLogger();
+
+    var fileName :- expect UUID.GenerateUUID();
+    assume {:axiom} metrics.ValidState();
+
+    var metricAgent := metrics.CreateTextMetricsAgent(
+      Types.CreateTextMetricsAgentInput(
+        fileName := fileName
+      )
+    );
+  }
+}
