Metrics/dafny/Metrics/Model/metrics-agent.smithy
@@ -1,0 +1,127 @@
+namespace aws.cryptography.metrics
+
+use aws.polymorph#reference
+use aws.polymorph#extendable
+
+@extendable
+resource MetricsAgent {
+  operations: [
+    PutDate,
+    PutTime,
+    PutCount,
+    PutProperty
+  ]
+}
+
+// Operations for different metric types
+operation PutDate {
+  input: PutDateInput,
+  output: PutOutput,
+  errors: [MetricsPutError]
+}
+
+operation PutTime {
+  input: PutTimeInput,
+  output: PutOutput,
+  errors: [MetricsPutError]
+}
+
+operation PutCount {
+  input: PutCountInput,
+  output: PutOutput,
+  errors: [MetricsPutError]
+}
+
+operation PutProperty {
+  input: PutPropertyInput,
+  output: PutOutput,
+  errors: [MetricsPutError]
+}
+
+// Input structures for each operation with flattened values
+structure PutDateInput {
+  @required
+  description: String,
+  @required
+  date: Timestamp,
+  transactionId: String
+}
+
+structure PutTimeInput {
+  @required
+  description: String,
+  @required
+  duration: Long,  // Duration in milliseconds
+  transactionId: String
+}
+
+structure PutCountInput {
+  @required
+  description: String,
+  @required
+  count: Long,
+  transactionId: String
+}
+
+structure PutPropertyInput {
+  @required
+  description: String,
+  @required
+  value: String,
+  transactionId: String
+}
+
+// Common output structure
+structure PutOutput {}
+
+@error("client")
+structure MetricsPutError {
+  @required
+  message: String,
+} 
+
+@error("client")
+structure MetricsPublishError {
+  @required
+  message: String
+}
+
+@error("client")
+structure MetricsServiceError {
+  @required
+  message: String
+}
+
+@reference(resource: MetricsAgent)
+structure MetricsAgentReference {}
+
+list MetricsAgentList {
+  member: MetricsAgentReference
+}
+
+// TextMetricsAgent Constructor
+operation CreateTextMetricsAgent {
+  input: CreateTextMetricsAgentInput,
+  output: CreateMetricsAgentOutput
+}
+
+structure CreateTextMetricsAgentInput {
+  @required
+  fileName: String
+}
+
+// MultiMetricsAgent Constructor
+operation CreateMultiMetricsAgent {
+    input: CreateMetricsAgentInput,
+    output: CreateMetricsAgentOutput
+}
+
+structure CreateMetricsAgentInput {
+    @required 
+    metricsAgents: MetricsAgentList
+}
+
+structure CreateMetricsAgentOutput {
+    @required
+    metricsAgent: MetricsAgentReference
+}
