Metrics/dafny/Metrics/Model/metrics.smithy
@@ -1,51 +1,25 @@
 namespace aws.cryptography.metrics
 
-use aws.polymorph#localService
 use aws.polymorph#reference
 use aws.polymorph#positional
 use aws.polymorph#extendable
 
 @aws.polymorph#localService(
-  sdkId: "MetricsLogger",
-  config: MetricsLoggerConfig
+  sdkId: "Metrics",
+  config: MetricsConfig
 )
 service AwsCryptographicMetrics {
   version: "2023-04-01",
-  resources: [Logger],
+  resources: [MetricsAgent],
   operations: [
-    CreateTextLogger,
-    // CreateAwsCloudWatchLogger
+    CreateTextMetricsAgent,
+    CreateMultiMetricsAgent
   ],
   errors: [
     MetricsPutError,
     MetricsPublishError,
-    MetricsChainError,
     MetricsServiceError
   ]
 }
 
-structure MetricsLoggerConfig {}
-
-@error("client")
-structure MetricsPutError {
-  @required
-  message: String,
-} 
-
-@error("client")
-structure MetricsChainError {
-  @required
-  message: String,
-}
-
-@error("client")
-structure MetricsPublishError {
-  @required
-  message: String
-}
-
-@error("client")
-structure MetricsServiceError {
-  @required
-  message: String
-}
+structure MetricsConfig {}
