Metrics/dafny/Metrics/runtimes/java/settings.gradle.kts
@@ -1,0 +1,11 @@
+// Copyright Amazon.com Inc. or its affiliates. All Rights Reserved.
+// SPDX-License-Identifier: Apache-2.0
+
+rootProject.name = "AwsCryptographyMetrics"
+
+includeBuild(File("../../../StandardLibrary/runtimes/java/")) {
+  name = "StandardLibrary"
+  dependencySubstitution {
+    substitute(module("software.amazon.cryptography:StandardLibrary")).using(project(":"))
+  }
+}
